Instances/Examples/VexLeaEcxRdiPlus5Fixture.lean
@@ -13,25 +13,33 @@ def block : Amd64Block :=
   mkAmd64Block [
       .wrTmp 2 (.get .rdi),
       .wrTmp 1 (.add64 (.tmp 2) (.const 0x5)),
-      .wrTmp 4 (.low32 (.tmp 1)),
-      .wrTmp 3 (.uext32 (.tmp 4)),
+      .wrTmp 4 (.narrow32 (.tmp 1)),
+      .wrTmp 3 (.zext64 (.tmp 4)),
       .put .rcx (.tmp 3)
     ] 0x400003
 
 def input : Amd64ConcreteState :=
-  mkAmd64State
+  mkAmd64StateCC
     0x0
     0xdeadbeefdeadbeef
     0x1122334455667788
     0x400000
+    0x0
+    0x0
+    0x0
+    0x0
     ByteMem.empty
 
 def expected : Amd64ConcreteState :=
-  mkAmd64State
+  mkAmd64StateCC
     0x0
     0x5566778d
     0x1122334455667788
     0x400003
+    0x0
+    0x0
+    0x0
+    0x0
     ByteMem.empty
 
 end Instances.Examples.VexLeaEcxRdiPlus5Fixture
